Progress toward compiling translate test correctly

src/TranslateTest.v
@@ -3,20 +3,19 @@ Require Prog.
 Require CCLProg.
 
 Import Prog.
+Require Import BasicProg.
+Require Import Bool.
 
-Definition add_tuple (nums: nat * nat * nat) : prog nat :=
-  n1 <- Ret (fst (fst nums));
-    n2 <- Ret (snd (fst nums));
-    n3 <- Ret (snd nums);
-    Ret (n1+n2+n3).
+Definition add_tuple (nums: nat * nat * nat) (b:bool) : prog nat :=
+  If (bool_dec b true) {
+       n1 <- Ret (fst (fst nums));
+       n2 <- Ret (snd (fst nums));
+       n3 <- Ret (snd nums);
+       Ret (n1+n2+n3)
+     } else {
+    v <- Read 0;
+    Ret 1
+  }.
 
-Definition add_tuple_concur (nums: nat * nat * nat) :=
-  translate (add_tuple nums) CCLProg.Locked empty_cache.
-
-Import CCLProg.
-
-Definition add_tuple_concur_raw (nums: nat * nat * nat) : cprog _ :=
-  n1 <- CCLProg.Ret (fst (fst nums));
-    n2 <- CCLProg.Ret (snd (fst nums));
-    n3 <- CCLProg.Ret (snd nums);
-    Ret (n1+n2+n3, empty_cache).
+Definition add_tuple_concur (nums: nat * nat * nat) (b:bool) :=
+  translate (add_tuple nums b) CCLProg.Locked empty_cache.
